DynamoDbEncryption/runtimes/net/Generated/JsonEncryptor/TypeConversion.cs
@@ -15,11 +15,6 @@ namespace AWS.Cryptography.DbEncryptionSDK.DynamoDb.Json
         converted.Crypto = FromDafny_N3_aws__N12_cryptography__N15_dbEncryptionSdk__N8_dynamoDb__N4_json__S6_Action__M6_crypto(concrete.dtor_crypto);
         return converted;
       }
-      if (value.is_esdk)
-      {
-        converted.Esdk = FromDafny_N3_aws__N12_cryptography__N15_dbEncryptionSdk__N8_dynamoDb__N4_json__S6_Action__M4_esdk(concrete.dtor_esdk);
-        return converted;
-      }
       if (value.is_dbesdk)
       {
         converted.Dbesdk = FromDafny_N3_aws__N12_cryptography__N15_dbEncryptionSdk__N8_dynamoDb__N4_json__S6_Action__M6_dbesdk(concrete.dtor_dbesdk);
@@ -32,10 +27,6 @@ namespace AWS.Cryptography.DbEncryptionSDK.DynamoDb.Json
       if (value.IsSetCrypto())
       {
         return software.amazon.cryptography.dbencryptionsdk.dynamodb.json.internaldafny.types.Action.create_crypto(ToDafny_N3_aws__N12_cryptography__N15_dbEncryptionSdk__N8_dynamoDb__N4_json__S6_Action__M6_crypto(value.Crypto));
-      }
-      if (value.IsSetEsdk())
-      {
-        return software.amazon.cryptography.dbencryptionsdk.dynamodb.json.internaldafny.types.Action.create_esdk(ToDafny_N3_aws__N12_cryptography__N15_dbEncryptionSdk__N8_dynamoDb__N4_json__S6_Action__M4_esdk(value.Esdk));
       }
       if (value.IsSetDbesdk())
       {
@@ -111,16 +102,16 @@ namespace AWS.Cryptography.DbEncryptionSDK.DynamoDb.Json
     public static AWS.Cryptography.DbEncryptionSDK.DynamoDb.Json.JsonEncryptorConfig FromDafny_N3_aws__N12_cryptography__N15_dbEncryptionSdk__N8_dynamoDb__N4_json__S19_JsonEncryptorConfig(software.amazon.cryptography.dbencryptionsdk.dynamodb.json.internaldafny.types._IJsonEncryptorConfig value)
     {
       software.amazon.cryptography.dbencryptionsdk.dynamodb.json.internaldafny.types.JsonEncryptorConfig concrete = (software.amazon.cryptography.dbencryptionsdk.dynamodb.json.internaldafny.types.JsonEncryptorConfig)value; AWS.Cryptography.DbEncryptionSDK.DynamoDb.Json.JsonEncryptorConfig converted = new AWS.Cryptography.DbEncryptionSDK.DynamoDb.Json.JsonEncryptorConfig(); converted.Domain = (string)FromDafny_N3_aws__N12_cryptography__N15_dbEncryptionSdk__N8_dynamoDb__N4_json__S19_JsonEncryptorConfig__M6_domain(concrete._domain);
-      converted.AttributeActionsOnEncrypt = (System.Collections.Generic.Dictionary<string, AWS.Cryptography.DbEncryptionSDK.DynamoDb.Json.Action>)FromDafny_N3_aws__N12_cryptography__N15_dbEncryptionSdk__N8_dynamoDb__N4_json__S19_JsonEncryptorConfig__M25_attributeActionsOnEncrypt(concrete._attributeActionsOnEncrypt);
-      if (concrete._allowedUnsignedAttributes.is_Some) converted.AllowedUnsignedAttributes = (System.Collections.Generic.List<string>)FromDafny_N3_aws__N12_cryptography__N15_dbEncryptionSdk__N8_dynamoDb__N4_json__S19_JsonEncryptorConfig__M25_allowedUnsignedAttributes(concrete._allowedUnsignedAttributes);
-      if (concrete._allowedUnsignedAttributePrefix.is_Some) converted.AllowedUnsignedAttributePrefix = (string)FromDafny_N3_aws__N12_cryptography__N15_dbEncryptionSdk__N8_dynamoDb__N4_json__S19_JsonEncryptorConfig__M30_allowedUnsignedAttributePrefix(concrete._allowedUnsignedAttributePrefix);
+      converted.MemberActionsOnEncrypt = (System.Collections.Generic.Dictionary<string, AWS.Cryptography.DbEncryptionSDK.DynamoDb.Json.Action>)FromDafny_N3_aws__N12_cryptography__N15_dbEncryptionSdk__N8_dynamoDb__N4_json__S19_JsonEncryptorConfig__M22_memberActionsOnEncrypt(concrete._memberActionsOnEncrypt);
+      if (concrete._allowedUnsignedMembers.is_Some) converted.AllowedUnsignedMembers = (System.Collections.Generic.List<string>)FromDafny_N3_aws__N12_cryptography__N15_dbEncryptionSdk__N8_dynamoDb__N4_json__S19_JsonEncryptorConfig__M22_allowedUnsignedMembers(concrete._allowedUnsignedMembers);
+      if (concrete._allowedUnsignedMemberPrefix.is_Some) converted.AllowedUnsignedMemberPrefix = (string)FromDafny_N3_aws__N12_cryptography__N15_dbEncryptionSdk__N8_dynamoDb__N4_json__S19_JsonEncryptorConfig__M27_allowedUnsignedMemberPrefix(concrete._allowedUnsignedMemberPrefix);
       converted.Encrypt = (AWS.Cryptography.DbEncryptionSDK.DynamoDb.Json.JsonEncrypt)FromDafny_N3_aws__N12_cryptography__N15_dbEncryptionSdk__N8_dynamoDb__N4_json__S19_JsonEncryptorConfig__M7_encrypt(concrete._encrypt); return converted;
     }
     public static software.amazon.cryptography.dbencryptionsdk.dynamodb.json.internaldafny.types._IJsonEncryptorConfig ToDafny_N3_aws__N12_cryptography__N15_dbEncryptionSdk__N8_dynamoDb__N4_json__S19_JsonEncryptorConfig(AWS.Cryptography.DbEncryptionSDK.DynamoDb.Json.JsonEncryptorConfig value)
     {
-      System.Collections.Generic.List<string> var_allowedUnsignedAttributes = value.IsSetAllowedUnsignedAttributes() ? value.AllowedUnsignedAttributes : (System.Collections.Generic.List<string>)null;
-      string var_allowedUnsignedAttributePrefix = value.IsSetAllowedUnsignedAttributePrefix() ? value.AllowedUnsignedAttributePrefix : (string)null;
-      return new software.amazon.cryptography.dbencryptionsdk.dynamodb.json.internaldafny.types.JsonEncryptorConfig(ToDafny_N3_aws__N12_cryptography__N15_dbEncryptionSdk__N8_dynamoDb__N4_json__S19_JsonEncryptorConfig__M6_domain(value.Domain), ToDafny_N3_aws__N12_cryptography__N15_dbEncryptionSdk__N8_dynamoDb__N4_json__S19_JsonEncryptorConfig__M25_attributeActionsOnEncrypt(value.AttributeActionsOnEncrypt), ToDafny_N3_aws__N12_cryptography__N15_dbEncryptionSdk__N8_dynamoDb__N4_json__S19_JsonEncryptorConfig__M25_allowedUnsignedAttributes(var_allowedUnsignedAttributes), ToDafny_N3_aws__N12_cryptography__N15_dbEncryptionSdk__N8_dynamoDb__N4_json__S19_JsonEncryptorConfig__M30_allowedUnsignedAttributePrefix(var_allowedUnsignedAttributePrefix), ToDafny_N3_aws__N12_cryptography__N15_dbEncryptionSdk__N8_dynamoDb__N4_json__S19_JsonEncryptorConfig__M7_encrypt(value.Encrypt));
+      System.Collections.Generic.List<string> var_allowedUnsignedMembers = value.IsSetAllowedUnsignedMembers() ? value.AllowedUnsignedMembers : (System.Collections.Generic.List<string>)null;
+      string var_allowedUnsignedMemberPrefix = value.IsSetAllowedUnsignedMemberPrefix() ? value.AllowedUnsignedMemberPrefix : (string)null;
+      return new software.amazon.cryptography.dbencryptionsdk.dynamodb.json.internaldafny.types.JsonEncryptorConfig(ToDafny_N3_aws__N12_cryptography__N15_dbEncryptionSdk__N8_dynamoDb__N4_json__S19_JsonEncryptorConfig__M6_domain(value.Domain), ToDafny_N3_aws__N12_cryptography__N15_dbEncryptionSdk__N8_dynamoDb__N4_json__S19_JsonEncryptorConfig__M22_memberActionsOnEncrypt(value.MemberActionsOnEncrypt), ToDafny_N3_aws__N12_cryptography__N15_dbEncryptionSdk__N8_dynamoDb__N4_json__S19_JsonEncryptorConfig__M22_allowedUnsignedMembers(var_allowedUnsignedMembers), ToDafny_N3_aws__N12_cryptography__N15_dbEncryptionSdk__N8_dynamoDb__N4_json__S19_JsonEncryptorConfig__M27_allowedUnsignedMemberPrefix(var_allowedUnsignedMemberPrefix), ToDafny_N3_aws__N12_cryptography__N15_dbEncryptionSdk__N8_dynamoDb__N4_json__S19_JsonEncryptorConfig__M7_encrypt(value.Encrypt));
     }
     public static AWS.Cryptography.DbEncryptionSDK.DynamoDb.Json.JsonEncryptorException FromDafny_N3_aws__N12_cryptography__N15_dbEncryptionSdk__N8_dynamoDb__N4_json__S22_JsonEncryptorException(software.amazon.cryptography.dbencryptionsdk.dynamodb.json.internaldafny.types.Error_JsonEncryptorException value)
     {
@@ -142,14 +133,6 @@ namespace AWS.Cryptography.DbEncryptionSDK.DynamoDb.Json
     public static software.amazon.cryptography.dbencryptionsdk.structuredencryption.internaldafny.types._ICryptoAction ToDafny_N3_aws__N12_cryptography__N15_dbEncryptionSdk__N8_dynamoDb__N4_json__S6_Action__M6_crypto(AWS.Cryptography.DbEncryptionSDK.StructuredEncryption.CryptoAction value)
     {
       return ToDafny_N3_aws__N12_cryptography__N15_dbEncryptionSdk__N20_structuredEncryption__S12_CryptoAction(value);
-    }
-    public static AWS.Cryptography.DbEncryptionSDK.DynamoDb.Json.EsdkEncrypt FromDafny_N3_aws__N12_cryptography__N15_dbEncryptionSdk__N8_dynamoDb__N4_json__S6_Action__M4_esdk(software.amazon.cryptography.dbencryptionsdk.dynamodb.json.internaldafny.types._IEsdkEncrypt value)
-    {
-      return FromDafny_N3_aws__N12_cryptography__N15_dbEncryptionSdk__N8_dynamoDb__N4_json__S11_EsdkEncrypt(value);
-    }
-    public static software.amazon.cryptography.dbencryptionsdk.dynamodb.json.internaldafny.types._IEsdkEncrypt ToDafny_N3_aws__N12_cryptography__N15_dbEncryptionSdk__N8_dynamoDb__N4_json__S6_Action__M4_esdk(AWS.Cryptography.DbEncryptionSDK.DynamoDb.Json.EsdkEncrypt value)
-    {
-      return ToDafny_N3_aws__N12_cryptography__N15_dbEncryptionSdk__N8_dynamoDb__N4_json__S11_EsdkEncrypt(value);
     }
     public static AWS.Cryptography.DbEncryptionSDK.DynamoDb.Json.JsonEncrypt FromDafny_N3_aws__N12_cryptography__N15_dbEncryptionSdk__N8_dynamoDb__N4_json__S6_Action__M6_dbesdk(software.amazon.cryptography.dbencryptionsdk.dynamodb.json.internaldafny.types._IJsonEncrypt value)
     {
@@ -231,27 +214,27 @@ namespace AWS.Cryptography.DbEncryptionSDK.DynamoDb.Json
     {
       return ToDafny_N6_smithy__N3_api__S6_String(value);
     }
-    public static System.Collections.Generic.Dictionary<string, AWS.Cryptography.DbEncryptionSDK.DynamoDb.Json.Action> FromDafny_N3_aws__N12_cryptography__N15_dbEncryptionSdk__N8_dynamoDb__N4_json__S19_JsonEncryptorConfig__M25_attributeActionsOnEncrypt(Dafny.IMap<Dafny.ISequence<char>, software.amazon.cryptography.dbencryptionsdk.dynamodb.json.internaldafny.types._IAction> value)
+    public static System.Collections.Generic.Dictionary<string, AWS.Cryptography.DbEncryptionSDK.DynamoDb.Json.Action> FromDafny_N3_aws__N12_cryptography__N15_dbEncryptionSdk__N8_dynamoDb__N4_json__S19_JsonEncryptorConfig__M22_memberActionsOnEncrypt(Dafny.IMap<Dafny.ISequence<char>, software.amazon.cryptography.dbencryptionsdk.dynamodb.json.internaldafny.types._IAction> value)
     {
-      return FromDafny_N3_aws__N12_cryptography__N15_dbEncryptionSdk__N8_dynamoDb__N4_json__S16_AttributeActions(value);
+      return FromDafny_N3_aws__N12_cryptography__N15_dbEncryptionSdk__N8_dynamoDb__N4_json__S13_MemberActions(value);
     }
-    public static Dafny.IMap<Dafny.ISequence<char>, software.amazon.cryptography.dbencryptionsdk.dynamodb.json.internaldafny.types._IAction> ToDafny_N3_aws__N12_cryptography__N15_dbEncryptionSdk__N8_dynamoDb__N4_json__S19_JsonEncryptorConfig__M25_attributeActionsOnEncrypt(System.Collections.Generic.Dictionary<string, AWS.Cryptography.DbEncryptionSDK.DynamoDb.Json.Action> value)
+    public static Dafny.IMap<Dafny.ISequence<char>, software.amazon.cryptography.dbencryptionsdk.dynamodb.json.internaldafny.types._IAction> ToDafny_N3_aws__N12_cryptography__N15_dbEncryptionSdk__N8_dynamoDb__N4_json__S19_JsonEncryptorConfig__M22_memberActionsOnEncrypt(System.Collections.Generic.Dictionary<string, AWS.Cryptography.DbEncryptionSDK.DynamoDb.Json.Action> value)
     {
-      return ToDafny_N3_aws__N12_cryptography__N15_dbEncryptionSdk__N8_dynamoDb__N4_json__S16_AttributeActions(value);
+      return ToDafny_N3_aws__N12_cryptography__N15_dbEncryptionSdk__N8_dynamoDb__N4_json__S13_MemberActions(value);
     }
-    public static System.Collections.Generic.List<string> FromDafny_N3_aws__N12_cryptography__N15_dbEncryptionSdk__N8_dynamoDb__N4_json__S19_JsonEncryptorConfig__M25_allowedUnsignedAttributes(Wrappers_Compile._IOption<Dafny.ISequence<Dafny.ISequence<char>>> value)
+    public static System.Collections.Generic.List<string> FromDafny_N3_aws__N12_cryptography__N15_dbEncryptionSdk__N8_dynamoDb__N4_json__S19_JsonEncryptorConfig__M22_allowedUnsignedMembers(Wrappers_Compile._IOption<Dafny.ISequence<Dafny.ISequence<char>>> value)
     {
-      return value.is_None ? (System.Collections.Generic.List<string>)null : FromDafny_N3_aws__N12_cryptography__N15_dbEncryptionSdk__N8_dynamoDb__N4_json__S17_AttributeNameList(value.Extract());
+      return value.is_None ? (System.Collections.Generic.List<string>)null : FromDafny_N3_aws__N12_cryptography__N15_dbEncryptionSdk__N8_dynamoDb__N4_json__S14_MemberNameList(value.Extract());
     }
-    public static Wrappers_Compile._IOption<Dafny.ISequence<Dafny.ISequence<char>>> ToDafny_N3_aws__N12_cryptography__N15_dbEncryptionSdk__N8_dynamoDb__N4_json__S19_JsonEncryptorConfig__M25_allowedUnsignedAttributes(System.Collections.Generic.List<string> value)
+    public static Wrappers_Compile._IOption<Dafny.ISequence<Dafny.ISequence<char>>> ToDafny_N3_aws__N12_cryptography__N15_dbEncryptionSdk__N8_dynamoDb__N4_json__S19_JsonEncryptorConfig__M22_allowedUnsignedMembers(System.Collections.Generic.List<string> value)
     {
-      return value == null ? Wrappers_Compile.Option<Dafny.ISequence<Dafny.ISequence<char>>>.create_None() : Wrappers_Compile.Option<Dafny.ISequence<Dafny.ISequence<char>>>.create_Some(ToDafny_N3_aws__N12_cryptography__N15_dbEncryptionSdk__N8_dynamoDb__N4_json__S17_AttributeNameList((System.Collections.Generic.List<string>)value));
+      return value == null ? Wrappers_Compile.Option<Dafny.ISequence<Dafny.ISequence<char>>>.create_None() : Wrappers_Compile.Option<Dafny.ISequence<Dafny.ISequence<char>>>.create_Some(ToDafny_N3_aws__N12_cryptography__N15_dbEncryptionSdk__N8_dynamoDb__N4_json__S14_MemberNameList((System.Collections.Generic.List<string>)value));
     }
-    public static string FromDafny_N3_aws__N12_cryptography__N15_dbEncryptionSdk__N8_dynamoDb__N4_json__S19_JsonEncryptorConfig__M30_allowedUnsignedAttributePrefix(Wrappers_Compile._IOption<Dafny.ISequence<char>> value)
+    public static string FromDafny_N3_aws__N12_cryptography__N15_dbEncryptionSdk__N8_dynamoDb__N4_json__S19_JsonEncryptorConfig__M27_allowedUnsignedMemberPrefix(Wrappers_Compile._IOption<Dafny.ISequence<char>> value)
     {
       return value.is_None ? (string)null : FromDafny_N6_smithy__N3_api__S6_String(value.Extract());
     }
-    public static Wrappers_Compile._IOption<Dafny.ISequence<char>> ToDafny_N3_aws__N12_cryptography__N15_dbEncryptionSdk__N8_dynamoDb__N4_json__S19_JsonEncryptorConfig__M30_allowedUnsignedAttributePrefix(string value)
+    public static Wrappers_Compile._IOption<Dafny.ISequence<char>> ToDafny_N3_aws__N12_cryptography__N15_dbEncryptionSdk__N8_dynamoDb__N4_json__S19_JsonEncryptorConfig__M27_allowedUnsignedMemberPrefix(string value)
     {
       return value == null ? Wrappers_Compile.Option<Dafny.ISequence<char>>.create_None() : Wrappers_Compile.Option<Dafny.ISequence<char>>.create_Some(ToDafny_N6_smithy__N3_api__S6_String((string)value));
     }
@@ -287,29 +270,11 @@ namespace AWS.Cryptography.DbEncryptionSDK.DynamoDb.Json
       if (AWS.Cryptography.DbEncryptionSDK.StructuredEncryption.CryptoAction.DO_NOTHING.Equals(value)) return software.amazon.cryptography.dbencryptionsdk.structuredencryption.internaldafny.types.CryptoAction.create_DO__NOTHING();
       throw new System.ArgumentException("Invalid AWS.Cryptography.DbEncryptionSDK.StructuredEncryption.CryptoAction value");
     }
-    public static AWS.Cryptography.DbEncryptionSDK.DynamoDb.Json.EsdkEncrypt FromDafny_N3_aws__N12_cryptography__N15_dbEncryptionSdk__N8_dynamoDb__N4_json__S11_EsdkEncrypt(software.amazon.cryptography.dbencryptionsdk.dynamodb.json.internaldafny.types._IEsdkEncrypt value)
-    {
-      software.amazon.cryptography.dbencryptionsdk.dynamodb.json.internaldafny.types.EsdkEncrypt concrete = (software.amazon.cryptography.dbencryptionsdk.dynamodb.json.internaldafny.types.EsdkEncrypt)value; AWS.Cryptography.DbEncryptionSDK.DynamoDb.Json.EsdkEncrypt converted = new AWS.Cryptography.DbEncryptionSDK.DynamoDb.Json.EsdkEncrypt(); if (concrete._encryptionContext.is_Some) converted.EncryptionContext = (System.Collections.Generic.Dictionary<string, string>)FromDafny_N3_aws__N12_cryptography__N15_dbEncryptionSdk__N8_dynamoDb__N4_json__S11_EsdkEncrypt__M17_encryptionContext(concrete._encryptionContext);
-      if (concrete._materialsManager.is_Some) converted.MaterialsManager = (AWS.Cryptography.MaterialProviders.ICryptographicMaterialsManager)FromDafny_N3_aws__N12_cryptography__N15_dbEncryptionSdk__N8_dynamoDb__N4_json__S11_EsdkEncrypt__M16_materialsManager(concrete._materialsManager);
-      if (concrete._keyring.is_Some) converted.Keyring = (AWS.Cryptography.MaterialProviders.IKeyring)FromDafny_N3_aws__N12_cryptography__N15_dbEncryptionSdk__N8_dynamoDb__N4_json__S11_EsdkEncrypt__M7_keyring(concrete._keyring);
-      if (concrete._algorithmSuiteId.is_Some) converted.AlgorithmSuiteId = (AWS.Cryptography.MaterialProviders.ESDKAlgorithmSuiteId)FromDafny_N3_aws__N12_cryptography__N15_dbEncryptionSdk__N8_dynamoDb__N4_json__S11_EsdkEncrypt__M16_algorithmSuiteId(concrete._algorithmSuiteId);
-      if (concrete._frameLength.is_Some) converted.FrameLength = (long)FromDafny_N3_aws__N12_cryptography__N15_dbEncryptionSdk__N8_dynamoDb__N4_json__S11_EsdkEncrypt__M11_frameLength(concrete._frameLength); return converted;
-    }
-    public static software.amazon.cryptography.dbencryptionsdk.dynamodb.json.internaldafny.types._IEsdkEncrypt ToDafny_N3_aws__N12_cryptography__N15_dbEncryptionSdk__N8_dynamoDb__N4_json__S11_EsdkEncrypt(AWS.Cryptography.DbEncryptionSDK.DynamoDb.Json.EsdkEncrypt value)
-    {
-      System.Collections.Generic.Dictionary<string, string> var_encryptionContext = value.IsSetEncryptionContext() ? value.EncryptionContext : (System.Collections.Generic.Dictionary<string, string>)null;
-      AWS.Cryptography.MaterialProviders.ICryptographicMaterialsManager var_materialsManager = value.IsSetMaterialsManager() ? value.MaterialsManager : (AWS.Cryptography.MaterialProviders.ICryptographicMaterialsManager)null;
-      AWS.Cryptography.MaterialProviders.IKeyring var_keyring = value.IsSetKeyring() ? value.Keyring : (AWS.Cryptography.MaterialProviders.IKeyring)null;
-      AWS.Cryptography.MaterialProviders.ESDKAlgorithmSuiteId var_algorithmSuiteId = value.IsSetAlgorithmSuiteId() ? value.AlgorithmSuiteId : (AWS.Cryptography.MaterialProviders.ESDKAlgorithmSuiteId)null;
-      long? var_frameLength = value.IsSetFrameLength() ? value.FrameLength : (long?)null;
-      return new software.amazon.cryptography.dbencryptionsdk.dynamodb.json.internaldafny.types.EsdkEncrypt(ToDafny_N3_aws__N12_cryptography__N15_dbEncryptionSdk__N8_dynamoDb__N4_json__S11_EsdkEncrypt__M17_encryptionContext(var_encryptionContext), ToDafny_N3_aws__N12_cryptography__N15_dbEncryptionSdk__N8_dynamoDb__N4_json__S11_EsdkEncrypt__M16_materialsManager(var_materialsManager), ToDafny_N3_aws__N12_cryptography__N15_dbEncryptionSdk__N8_dynamoDb__N4_json__S11_EsdkEncrypt__M7_keyring(var_keyring), ToDafny_N3_aws__N12_cryptography__N15_dbEncryptionSdk__N8_dynamoDb__N4_json__S11_EsdkEncrypt__M16_algorithmSuiteId(var_algorithmSuiteId), ToDafny_N3_aws__N12_cryptography__N15_dbEncryptionSdk__N8_dynamoDb__N4_json__S11_EsdkEncrypt__M11_frameLength(var_frameLength));
-    }
     public static AWS.Cryptography.DbEncryptionSDK.DynamoDb.Json.JsonEncrypt FromDafny_N3_aws__N12_cryptography__N15_dbEncryptionSdk__N8_dynamoDb__N4_json__S11_JsonEncrypt(software.amazon.cryptography.dbencryptionsdk.dynamodb.json.internaldafny.types._IJsonEncrypt value)
     {
       software.amazon.cryptography.dbencryptionsdk.dynamodb.json.internaldafny.types.JsonEncrypt concrete = (software.amazon.cryptography.dbencryptionsdk.dynamodb.json.internaldafny.types.JsonEncrypt)value; AWS.Cryptography.DbEncryptionSDK.DynamoDb.Json.JsonEncrypt converted = new AWS.Cryptography.DbEncryptionSDK.DynamoDb.Json.JsonEncrypt(); if (concrete._keyring.is_Some) converted.Keyring = (AWS.Cryptography.MaterialProviders.IKeyring)FromDafny_N3_aws__N12_cryptography__N15_dbEncryptionSdk__N8_dynamoDb__N4_json__S11_JsonEncrypt__M7_keyring(concrete._keyring);
       if (concrete._cmm.is_Some) converted.Cmm = (AWS.Cryptography.MaterialProviders.ICryptographicMaterialsManager)FromDafny_N3_aws__N12_cryptography__N15_dbEncryptionSdk__N8_dynamoDb__N4_json__S11_JsonEncrypt__M3_cmm(concrete._cmm);
       if (concrete._algorithmSuiteId.is_Some) converted.AlgorithmSuiteId = (AWS.Cryptography.MaterialProviders.DBEAlgorithmSuiteId)FromDafny_N3_aws__N12_cryptography__N15_dbEncryptionSdk__N8_dynamoDb__N4_json__S11_JsonEncrypt__M16_algorithmSuiteId(concrete._algorithmSuiteId);
-      if (concrete._signedValue.is_Some) converted.SignedValue = (System.Collections.Generic.Dictionary<string, string>)FromDafny_N3_aws__N12_cryptography__N15_dbEncryptionSdk__N8_dynamoDb__N4_json__S11_JsonEncrypt__M11_signedValue(concrete._signedValue);
       if (concrete._encryptionContext.is_Some) converted.EncryptionContext = (System.Collections.Generic.Dictionary<string, string>)FromDafny_N3_aws__N12_cryptography__N15_dbEncryptionSdk__N8_dynamoDb__N4_json__S11_JsonEncrypt__M17_encryptionContext(concrete._encryptionContext); return converted;
     }
     public static software.amazon.cryptography.dbencryptionsdk.dynamodb.json.internaldafny.types._IJsonEncrypt ToDafny_N3_aws__N12_cryptography__N15_dbEncryptionSdk__N8_dynamoDb__N4_json__S11_JsonEncrypt(AWS.Cryptography.DbEncryptionSDK.DynamoDb.Json.JsonEncrypt value)
@@ -317,13 +282,12 @@ namespace AWS.Cryptography.DbEncryptionSDK.DynamoDb.Json
       AWS.Cryptography.MaterialProviders.IKeyring var_keyring = value.IsSetKeyring() ? value.Keyring : (AWS.Cryptography.MaterialProviders.IKeyring)null;
       AWS.Cryptography.MaterialProviders.ICryptographicMaterialsManager var_cmm = value.IsSetCmm() ? value.Cmm : (AWS.Cryptography.MaterialProviders.ICryptographicMaterialsManager)null;
       AWS.Cryptography.MaterialProviders.DBEAlgorithmSuiteId var_algorithmSuiteId = value.IsSetAlgorithmSuiteId() ? value.AlgorithmSuiteId : (AWS.Cryptography.MaterialProviders.DBEAlgorithmSuiteId)null;
-      System.Collections.Generic.Dictionary<string, string> var_signedValue = value.IsSetSignedValue() ? value.SignedValue : (System.Collections.Generic.Dictionary<string, string>)null;
       System.Collections.Generic.Dictionary<string, string> var_encryptionContext = value.IsSetEncryptionContext() ? value.EncryptionContext : (System.Collections.Generic.Dictionary<string, string>)null;
-      return new software.amazon.cryptography.dbencryptionsdk.dynamodb.json.internaldafny.types.JsonEncrypt(ToDafny_N3_aws__N12_cryptography__N15_dbEncryptionSdk__N8_dynamoDb__N4_json__S11_JsonEncrypt__M7_keyring(var_keyring), ToDafny_N3_aws__N12_cryptography__N15_dbEncryptionSdk__N8_dynamoDb__N4_json__S11_JsonEncrypt__M3_cmm(var_cmm), ToDafny_N3_aws__N12_cryptography__N15_dbEncryptionSdk__N8_dynamoDb__N4_json__S11_JsonEncrypt__M16_algorithmSuiteId(var_algorithmSuiteId), ToDafny_N3_aws__N12_cryptography__N15_dbEncryptionSdk__N8_dynamoDb__N4_json__S11_JsonEncrypt__M11_signedValue(var_signedValue), ToDafny_N3_aws__N12_cryptography__N15_dbEncryptionSdk__N8_dynamoDb__N4_json__S11_JsonEncrypt__M17_encryptionContext(var_encryptionContext));
+      return new software.amazon.cryptography.dbencryptionsdk.dynamodb.json.internaldafny.types.JsonEncrypt(ToDafny_N3_aws__N12_cryptography__N15_dbEncryptionSdk__N8_dynamoDb__N4_json__S11_JsonEncrypt__M7_keyring(var_keyring), ToDafny_N3_aws__N12_cryptography__N15_dbEncryptionSdk__N8_dynamoDb__N4_json__S11_JsonEncrypt__M3_cmm(var_cmm), ToDafny_N3_aws__N12_cryptography__N15_dbEncryptionSdk__N8_dynamoDb__N4_json__S11_JsonEncrypt__M16_algorithmSuiteId(var_algorithmSuiteId), ToDafny_N3_aws__N12_cryptography__N15_dbEncryptionSdk__N8_dynamoDb__N4_json__S11_JsonEncrypt__M17_encryptionContext(var_encryptionContext));
     }
     public static AWS.Cryptography.DbEncryptionSDK.DynamoDb.Json.ParsedHeader FromDafny_N3_aws__N12_cryptography__N15_dbEncryptionSdk__N8_dynamoDb__N4_json__S12_ParsedHeader(software.amazon.cryptography.dbencryptionsdk.dynamodb.json.internaldafny.types._IParsedHeader value)
     {
-      software.amazon.cryptography.dbencryptionsdk.dynamodb.json.internaldafny.types.ParsedHeader concrete = (software.amazon.cryptography.dbencryptionsdk.dynamodb.json.internaldafny.types.ParsedHeader)value; AWS.Cryptography.DbEncryptionSDK.DynamoDb.Json.ParsedHeader converted = new AWS.Cryptography.DbEncryptionSDK.DynamoDb.Json.ParsedHeader(); converted.AttributeActionsOnEncrypt = (System.Collections.Generic.Dictionary<string, AWS.Cryptography.DbEncryptionSDK.DynamoDb.Json.Action>)FromDafny_N3_aws__N12_cryptography__N15_dbEncryptionSdk__N8_dynamoDb__N4_json__S12_ParsedHeader__M25_attributeActionsOnEncrypt(concrete._attributeActionsOnEncrypt);
+      software.amazon.cryptography.dbencryptionsdk.dynamodb.json.internaldafny.types.ParsedHeader concrete = (software.amazon.cryptography.dbencryptionsdk.dynamodb.json.internaldafny.types.ParsedHeader)value; AWS.Cryptography.DbEncryptionSDK.DynamoDb.Json.ParsedHeader converted = new AWS.Cryptography.DbEncryptionSDK.DynamoDb.Json.ParsedHeader(); converted.MemberActionsOnEncrypt = (System.Collections.Generic.Dictionary<string, AWS.Cryptography.DbEncryptionSDK.DynamoDb.Json.Action>)FromDafny_N3_aws__N12_cryptography__N15_dbEncryptionSdk__N8_dynamoDb__N4_json__S12_ParsedHeader__M22_memberActionsOnEncrypt(concrete._memberActionsOnEncrypt);
       converted.AlgorithmSuiteId = (AWS.Cryptography.MaterialProviders.DBEAlgorithmSuiteId)FromDafny_N3_aws__N12_cryptography__N15_dbEncryptionSdk__N8_dynamoDb__N4_json__S12_ParsedHeader__M16_algorithmSuiteId(concrete._algorithmSuiteId);
       converted.EncryptedDataKeys = (System.Collections.Generic.List<AWS.Cryptography.MaterialProviders.EncryptedDataKey>)FromDafny_N3_aws__N12_cryptography__N15_dbEncryptionSdk__N8_dynamoDb__N4_json__S12_ParsedHeader__M17_encryptedDataKeys(concrete._encryptedDataKeys);
       converted.StoredEncryptionContext = (System.Collections.Generic.Dictionary<string, string>)FromDafny_N3_aws__N12_cryptography__N15_dbEncryptionSdk__N8_dynamoDb__N4_json__S12_ParsedHeader__M23_storedEncryptionContext(concrete._storedEncryptionContext);
@@ -332,7 +296,7 @@ namespace AWS.Cryptography.DbEncryptionSDK.DynamoDb.Json
     public static software.amazon.cryptography.dbencryptionsdk.dynamodb.json.internaldafny.types._IParsedHeader ToDafny_N3_aws__N12_cryptography__N15_dbEncryptionSdk__N8_dynamoDb__N4_json__S12_ParsedHeader(AWS.Cryptography.DbEncryptionSDK.DynamoDb.Json.ParsedHeader value)
     {
 
-      return new software.amazon.cryptography.dbencryptionsdk.dynamodb.json.internaldafny.types.ParsedHeader(ToDafny_N3_aws__N12_cryptography__N15_dbEncryptionSdk__N8_dynamoDb__N4_json__S12_ParsedHeader__M25_attributeActionsOnEncrypt(value.AttributeActionsOnEncrypt), ToDafny_N3_aws__N12_cryptography__N15_dbEncryptionSdk__N8_dynamoDb__N4_json__S12_ParsedHeader__M16_algorithmSuiteId(value.AlgorithmSuiteId), ToDafny_N3_aws__N12_cryptography__N15_dbEncryptionSdk__N8_dynamoDb__N4_json__S12_ParsedHeader__M17_encryptedDataKeys(value.EncryptedDataKeys), ToDafny_N3_aws__N12_cryptography__N15_dbEncryptionSdk__N8_dynamoDb__N4_json__S12_ParsedHeader__M23_storedEncryptionContext(value.StoredEncryptionContext), ToDafny_N3_aws__N12_cryptography__N15_dbEncryptionSdk__N8_dynamoDb__N4_json__S12_ParsedHeader__M17_encryptionContext(value.EncryptionContext));
+      return new software.amazon.cryptography.dbencryptionsdk.dynamodb.json.internaldafny.types.ParsedHeader(ToDafny_N3_aws__N12_cryptography__N15_dbEncryptionSdk__N8_dynamoDb__N4_json__S12_ParsedHeader__M22_memberActionsOnEncrypt(value.MemberActionsOnEncrypt), ToDafny_N3_aws__N12_cryptography__N15_dbEncryptionSdk__N8_dynamoDb__N4_json__S12_ParsedHeader__M16_algorithmSuiteId(value.AlgorithmSuiteId), ToDafny_N3_aws__N12_cryptography__N15_dbEncryptionSdk__N8_dynamoDb__N4_json__S12_ParsedHeader__M17_encryptedDataKeys(value.EncryptedDataKeys), ToDafny_N3_aws__N12_cryptography__N15_dbEncryptionSdk__N8_dynamoDb__N4_json__S12_ParsedHeader__M23_storedEncryptionContext(value.StoredEncryptionContext), ToDafny_N3_aws__N12_cryptography__N15_dbEncryptionSdk__N8_dynamoDb__N4_json__S12_ParsedHeader__M17_encryptionContext(value.EncryptionContext));
     }
     public static string FromDafny_N3_aws__N12_cryptography__N15_dbEncryptionSdk__N8_dynamoDb__N4_json__S9_Utf8Bytes(Dafny.ISequence<byte> value)
     {
@@ -352,63 +316,23 @@ namespace AWS.Cryptography.DbEncryptionSDK.DynamoDb.Json
     {
       return Dafny.Sequence<char>.FromString(value);
     }
-    public static System.Collections.Generic.Dictionary<string, AWS.Cryptography.DbEncryptionSDK.DynamoDb.Json.Action> FromDafny_N3_aws__N12_cryptography__N15_dbEncryptionSdk__N8_dynamoDb__N4_json__S16_AttributeActions(Dafny.IMap<Dafny.ISequence<char>, software.amazon.cryptography.dbencryptionsdk.dynamodb.json.internaldafny.types._IAction> value)
+    public static System.Collections.Generic.Dictionary<string, AWS.Cryptography.DbEncryptionSDK.DynamoDb.Json.Action> FromDafny_N3_aws__N12_cryptography__N15_dbEncryptionSdk__N8_dynamoDb__N4_json__S13_MemberActions(Dafny.IMap<Dafny.ISequence<char>, software.amazon.cryptography.dbencryptionsdk.dynamodb.json.internaldafny.types._IAction> value)
     {
-      return value.ItemEnumerable.ToDictionary(pair => FromDafny_N3_aws__N12_cryptography__N15_dbEncryptionSdk__N8_dynamoDb__N4_json__S16_AttributeActions__M3_key(pair.Car), pair => FromDafny_N3_aws__N12_cryptography__N15_dbEncryptionSdk__N8_dynamoDb__N4_json__S16_AttributeActions__M5_value(pair.Cdr));
+      return value.ItemEnumerable.ToDictionary(pair => FromDafny_N3_aws__N12_cryptography__N15_dbEncryptionSdk__N8_dynamoDb__N4_json__S13_MemberActions__M3_key(pair.Car), pair => FromDafny_N3_aws__N12_cryptography__N15_dbEncryptionSdk__N8_dynamoDb__N4_json__S13_MemberActions__M5_value(pair.Cdr));
     }
-    public static Dafny.IMap<Dafny.ISequence<char>, software.amazon.cryptography.dbencryptionsdk.dynamodb.json.internaldafny.types._IAction> ToDafny_N3_aws__N12_cryptography__N15_dbEncryptionSdk__N8_dynamoDb__N4_json__S16_AttributeActions(System.Collections.Generic.Dictionary<string, AWS.Cryptography.DbEncryptionSDK.DynamoDb.Json.Action> value)
+    public static Dafny.IMap<Dafny.ISequence<char>, software.amazon.cryptography.dbencryptionsdk.dynamodb.json.internaldafny.types._IAction> ToDafny_N3_aws__N12_cryptography__N15_dbEncryptionSdk__N8_dynamoDb__N4_json__S13_MemberActions(System.Collections.Generic.Dictionary<string, AWS.Cryptography.DbEncryptionSDK.DynamoDb.Json.Action> value)
     {
       return Dafny.Map<Dafny.ISequence<char>, software.amazon.cryptography.dbencryptionsdk.dynamodb.json.internaldafny.types._IAction>.FromCollection(value.Select(pair =>
-         new Dafny.Pair<Dafny.ISequence<char>, software.amazon.cryptography.dbencryptionsdk.dynamodb.json.internaldafny.types._IAction>(ToDafny_N3_aws__N12_cryptography__N15_dbEncryptionSdk__N8_dynamoDb__N4_json__S16_AttributeActions__M3_key(pair.Key), ToDafny_N3_aws__N12_cryptography__N15_dbEncryptionSdk__N8_dynamoDb__N4_json__S16_AttributeActions__M5_value(pair.Value))
+         new Dafny.Pair<Dafny.ISequence<char>, software.amazon.cryptography.dbencryptionsdk.dynamodb.json.internaldafny.types._IAction>(ToDafny_N3_aws__N12_cryptography__N15_dbEncryptionSdk__N8_dynamoDb__N4_json__S13_MemberActions__M3_key(pair.Key), ToDafny_N3_aws__N12_cryptography__N15_dbEncryptionSdk__N8_dynamoDb__N4_json__S13_MemberActions__M5_value(pair.Value))
      ));
     }
-    public static System.Collections.Generic.List<string> FromDafny_N3_aws__N12_cryptography__N15_dbEncryptionSdk__N8_dynamoDb__N4_json__S17_AttributeNameList(Dafny.ISequence<Dafny.ISequence<char>> value)
+    public static System.Collections.Generic.List<string> FromDafny_N3_aws__N12_cryptography__N15_dbEncryptionSdk__N8_dynamoDb__N4_json__S14_MemberNameList(Dafny.ISequence<Dafny.ISequence<char>> value)
     {
-      return new System.Collections.Generic.List<string>(value.Elements.Select(FromDafny_N3_aws__N12_cryptography__N15_dbEncryptionSdk__N8_dynamoDb__N4_json__S17_AttributeNameList__M6_member));
+      return new System.Collections.Generic.List<string>(value.Elements.Select(FromDafny_N3_aws__N12_cryptography__N15_dbEncryptionSdk__N8_dynamoDb__N4_json__S14_MemberNameList__M6_member));
     }
-    public static Dafny.ISequence<Dafny.ISequence<char>> ToDafny_N3_aws__N12_cryptography__N15_dbEncryptionSdk__N8_dynamoDb__N4_json__S17_AttributeNameList(System.Collections.Generic.List<string> value)
+    public static Dafny.ISequence<Dafny.ISequence<char>> ToDafny_N3_aws__N12_cryptography__N15_dbEncryptionSdk__N8_dynamoDb__N4_json__S14_MemberNameList(System.Collections.Generic.List<string> value)
     {
-      return Dafny.Sequence<Dafny.ISequence<char>>.FromArray(value.Select(ToDafny_N3_aws__N12_cryptography__N15_dbEncryptionSdk__N8_dynamoDb__N4_json__S17_AttributeNameList__M6_member).ToArray());
-    }
-    public static System.Collections.Generic.Dictionary<string, string> FromDafny_N3_aws__N12_cryptography__N15_dbEncryptionSdk__N8_dynamoDb__N4_json__S11_EsdkEncrypt__M17_encryptionContext(Wrappers_Compile._IOption<Dafny.IMap<Dafny.ISequence<byte>, Dafny.ISequence<byte>>> value)
-    {
-      return value.is_None ? (System.Collections.Generic.Dictionary<string, string>)null : FromDafny_N3_aws__N12_cryptography__N17_materialProviders__S17_EncryptionContext(value.Extract());
-    }
-    public static Wrappers_Compile._IOption<Dafny.IMap<Dafny.ISequence<byte>, Dafny.ISequence<byte>>> ToDafny_N3_aws__N12_cryptography__N15_dbEncryptionSdk__N8_dynamoDb__N4_json__S11_EsdkEncrypt__M17_encryptionContext(System.Collections.Generic.Dictionary<string, string> value)
-    {
-      return value == null ? Wrappers_Compile.Option<Dafny.IMap<Dafny.ISequence<byte>, Dafny.ISequence<byte>>>.create_None() : Wrappers_Compile.Option<Dafny.IMap<Dafny.ISequence<byte>, Dafny.ISequence<byte>>>.create_Some(ToDafny_N3_aws__N12_cryptography__N17_materialProviders__S17_EncryptionContext((System.Collections.Generic.Dictionary<string, string>)value));
-    }
-    public static AWS.Cryptography.MaterialProviders.ICryptographicMaterialsManager FromDafny_N3_aws__N12_cryptography__N15_dbEncryptionSdk__N8_dynamoDb__N4_json__S11_EsdkEncrypt__M16_materialsManager(Wrappers_Compile._IOption<software.amazon.cryptography.materialproviders.internaldafny.types.ICryptographicMaterialsManager> value)
-    {
-      return value.is_None ? (AWS.Cryptography.MaterialProviders.ICryptographicMaterialsManager)null : FromDafny_N3_aws__N12_cryptography__N17_materialProviders__S38_CryptographicMaterialsManagerReference(value.Extract());
-    }
-    public static Wrappers_Compile._IOption<software.amazon.cryptography.materialproviders.internaldafny.types.ICryptographicMaterialsManager> ToDafny_N3_aws__N12_cryptography__N15_dbEncryptionSdk__N8_dynamoDb__N4_json__S11_EsdkEncrypt__M16_materialsManager(AWS.Cryptography.MaterialProviders.ICryptographicMaterialsManager value)
-    {
-      return value == null ? Wrappers_Compile.Option<software.amazon.cryptography.materialproviders.internaldafny.types.ICryptographicMaterialsManager>.create_None() : Wrappers_Compile.Option<software.amazon.cryptography.materialproviders.internaldafny.types.ICryptographicMaterialsManager>.create_Some(ToDafny_N3_aws__N12_cryptography__N17_materialProviders__S38_CryptographicMaterialsManagerReference((AWS.Cryptography.MaterialProviders.ICryptographicMaterialsManager)value));
-    }
-    public static AWS.Cryptography.MaterialProviders.IKeyring FromDafny_N3_aws__N12_cryptography__N15_dbEncryptionSdk__N8_dynamoDb__N4_json__S11_EsdkEncrypt__M7_keyring(Wrappers_Compile._IOption<software.amazon.cryptography.materialproviders.internaldafny.types.IKeyring> value)
-    {
-      return value.is_None ? (AWS.Cryptography.MaterialProviders.IKeyring)null : FromDafny_N3_aws__N12_cryptography__N17_materialProviders__S16_KeyringReference(value.Extract());
-    }
-    public static Wrappers_Compile._IOption<software.amazon.cryptography.materialproviders.internaldafny.types.IKeyring> ToDafny_N3_aws__N12_cryptography__N15_dbEncryptionSdk__N8_dynamoDb__N4_json__S11_EsdkEncrypt__M7_keyring(AWS.Cryptography.MaterialProviders.IKeyring value)
-    {
-      return value == null ? Wrappers_Compile.Option<software.amazon.cryptography.materialproviders.internaldafny.types.IKeyring>.create_None() : Wrappers_Compile.Option<software.amazon.cryptography.materialproviders.internaldafny.types.IKeyring>.create_Some(ToDafny_N3_aws__N12_cryptography__N17_materialProviders__S16_KeyringReference((AWS.Cryptography.MaterialProviders.IKeyring)value));
-    }
-    public static AWS.Cryptography.MaterialProviders.ESDKAlgorithmSuiteId FromDafny_N3_aws__N12_cryptography__N15_dbEncryptionSdk__N8_dynamoDb__N4_json__S11_EsdkEncrypt__M16_algorithmSuiteId(Wrappers_Compile._IOption<software.amazon.cryptography.materialproviders.internaldafny.types._IESDKAlgorithmSuiteId> value)
-    {
-      return value.is_None ? (AWS.Cryptography.MaterialProviders.ESDKAlgorithmSuiteId)null : FromDafny_N3_aws__N12_cryptography__N17_materialProviders__S20_ESDKAlgorithmSuiteId(value.Extract());
-    }
-    public static Wrappers_Compile._IOption<software.amazon.cryptography.materialproviders.internaldafny.types._IESDKAlgorithmSuiteId> ToDafny_N3_aws__N12_cryptography__N15_dbEncryptionSdk__N8_dynamoDb__N4_json__S11_EsdkEncrypt__M16_algorithmSuiteId(AWS.Cryptography.MaterialProviders.ESDKAlgorithmSuiteId value)
-    {
-      return value == null ? Wrappers_Compile.Option<software.amazon.cryptography.materialproviders.internaldafny.types._IESDKAlgorithmSuiteId>.create_None() : Wrappers_Compile.Option<software.amazon.cryptography.materialproviders.internaldafny.types._IESDKAlgorithmSuiteId>.create_Some(ToDafny_N3_aws__N12_cryptography__N17_materialProviders__S20_ESDKAlgorithmSuiteId((AWS.Cryptography.MaterialProviders.ESDKAlgorithmSuiteId)value));
-    }
-    public static long? FromDafny_N3_aws__N12_cryptography__N15_dbEncryptionSdk__N8_dynamoDb__N4_json__S11_EsdkEncrypt__M11_frameLength(Wrappers_Compile._IOption<long> value)
-    {
-      return value.is_None ? (long?)null : FromDafny_N3_aws__N12_cryptography__N15_dbEncryptionSdk__N8_dynamoDb__N4_json__S11_FrameLength(value.Extract());
-    }
-    public static Wrappers_Compile._IOption<long> ToDafny_N3_aws__N12_cryptography__N15_dbEncryptionSdk__N8_dynamoDb__N4_json__S11_EsdkEncrypt__M11_frameLength(long? value)
-    {
-      return value == null ? Wrappers_Compile.Option<long>.create_None() : Wrappers_Compile.Option<long>.create_Some(ToDafny_N3_aws__N12_cryptography__N15_dbEncryptionSdk__N8_dynamoDb__N4_json__S11_FrameLength((long)value));
+      return Dafny.Sequence<Dafny.ISequence<char>>.FromArray(value.Select(ToDafny_N3_aws__N12_cryptography__N15_dbEncryptionSdk__N8_dynamoDb__N4_json__S14_MemberNameList__M6_member).ToArray());
     }
     public static AWS.Cryptography.MaterialProviders.IKeyring FromDafny_N3_aws__N12_cryptography__N15_dbEncryptionSdk__N8_dynamoDb__N4_json__S11_JsonEncrypt__M7_keyring(Wrappers_Compile._IOption<software.amazon.cryptography.materialproviders.internaldafny.types.IKeyring> value)
     {
@@ -434,14 +358,6 @@ namespace AWS.Cryptography.DbEncryptionSDK.DynamoDb.Json
     {
       return value == null ? Wrappers_Compile.Option<software.amazon.cryptography.materialproviders.internaldafny.types._IDBEAlgorithmSuiteId>.create_None() : Wrappers_Compile.Option<software.amazon.cryptography.materialproviders.internaldafny.types._IDBEAlgorithmSuiteId>.create_Some(ToDafny_N3_aws__N12_cryptography__N17_materialProviders__S19_DBEAlgorithmSuiteId((AWS.Cryptography.MaterialProviders.DBEAlgorithmSuiteId)value));
     }
-    public static System.Collections.Generic.Dictionary<string, string> FromDafny_N3_aws__N12_cryptography__N15_dbEncryptionSdk__N8_dynamoDb__N4_json__S11_JsonEncrypt__M11_signedValue(Wrappers_Compile._IOption<Dafny.IMap<Dafny.ISequence<char>, Dafny.ISequence<char>>> value)
-    {
-      return value.is_None ? (System.Collections.Generic.Dictionary<string, string>)null : FromDafny_N3_aws__N12_cryptography__N15_dbEncryptionSdk__N8_dynamoDb__N4_json__S12_SignedValues(value.Extract());
-    }
-    public static Wrappers_Compile._IOption<Dafny.IMap<Dafny.ISequence<char>, Dafny.ISequence<char>>> ToDafny_N3_aws__N12_cryptography__N15_dbEncryptionSdk__N8_dynamoDb__N4_json__S11_JsonEncrypt__M11_signedValue(System.Collections.Generic.Dictionary<string, string> value)
-    {
-      return value == null ? Wrappers_Compile.Option<Dafny.IMap<Dafny.ISequence<char>, Dafny.ISequence<char>>>.create_None() : Wrappers_Compile.Option<Dafny.IMap<Dafny.ISequence<char>, Dafny.ISequence<char>>>.create_Some(ToDafny_N3_aws__N12_cryptography__N15_dbEncryptionSdk__N8_dynamoDb__N4_json__S12_SignedValues((System.Collections.Generic.Dictionary<string, string>)value));
-    }
     public static System.Collections.Generic.Dictionary<string, string> FromDafny_N3_aws__N12_cryptography__N15_dbEncryptionSdk__N8_dynamoDb__N4_json__S11_JsonEncrypt__M17_encryptionContext(Wrappers_Compile._IOption<Dafny.IMap<Dafny.ISequence<byte>, Dafny.ISequence<byte>>> value)
     {
       return value.is_None ? (System.Collections.Generic.Dictionary<string, string>)null : FromDafny_N3_aws__N12_cryptography__N17_materialProviders__S17_EncryptionContext(value.Extract());
@@ -450,13 +366,13 @@ namespace AWS.Cryptography.DbEncryptionSDK.DynamoDb.Json
     {
       return value == null ? Wrappers_Compile.Option<Dafny.IMap<Dafny.ISequence<byte>, Dafny.ISequence<byte>>>.create_None() : Wrappers_Compile.Option<Dafny.IMap<Dafny.ISequence<byte>, Dafny.ISequence<byte>>>.create_Some(ToDafny_N3_aws__N12_cryptography__N17_materialProviders__S17_EncryptionContext((System.Collections.Generic.Dictionary<string, string>)value));
     }
-    public static System.Collections.Generic.Dictionary<string, AWS.Cryptography.DbEncryptionSDK.DynamoDb.Json.Action> FromDafny_N3_aws__N12_cryptography__N15_dbEncryptionSdk__N8_dynamoDb__N4_json__S12_ParsedHeader__M25_attributeActionsOnEncrypt(Dafny.IMap<Dafny.ISequence<char>, software.amazon.cryptography.dbencryptionsdk.dynamodb.json.internaldafny.types._IAction> value)
+    public static System.Collections.Generic.Dictionary<string, AWS.Cryptography.DbEncryptionSDK.DynamoDb.Json.Action> FromDafny_N3_aws__N12_cryptography__N15_dbEncryptionSdk__N8_dynamoDb__N4_json__S12_ParsedHeader__M22_memberActionsOnEncrypt(Dafny.IMap<Dafny.ISequence<char>, software.amazon.cryptography.dbencryptionsdk.dynamodb.json.internaldafny.types._IAction> value)
     {
-      return FromDafny_N3_aws__N12_cryptography__N15_dbEncryptionSdk__N8_dynamoDb__N4_json__S16_AttributeActions(value);
+      return FromDafny_N3_aws__N12_cryptography__N15_dbEncryptionSdk__N8_dynamoDb__N4_json__S13_MemberActions(value);
     }
-    public static Dafny.IMap<Dafny.ISequence<char>, software.amazon.cryptography.dbencryptionsdk.dynamodb.json.internaldafny.types._IAction> ToDafny_N3_aws__N12_cryptography__N15_dbEncryptionSdk__N8_dynamoDb__N4_json__S12_ParsedHeader__M25_attributeActionsOnEncrypt(System.Collections.Generic.Dictionary<string, AWS.Cryptography.DbEncryptionSDK.DynamoDb.Json.Action> value)
+    public static Dafny.IMap<Dafny.ISequence<char>, software.amazon.cryptography.dbencryptionsdk.dynamodb.json.internaldafny.types._IAction> ToDafny_N3_aws__N12_cryptography__N15_dbEncryptionSdk__N8_dynamoDb__N4_json__S12_ParsedHeader__M22_memberActionsOnEncrypt(System.Collections.Generic.Dictionary<string, AWS.Cryptography.DbEncryptionSDK.DynamoDb.Json.Action> value)
     {
-      return ToDafny_N3_aws__N12_cryptography__N15_dbEncryptionSdk__N8_dynamoDb__N4_json__S16_AttributeActions(value);
+      return ToDafny_N3_aws__N12_cryptography__N15_dbEncryptionSdk__N8_dynamoDb__N4_json__S13_MemberActions(value);
     }
     public static AWS.Cryptography.MaterialProviders.DBEAlgorithmSuiteId FromDafny_N3_aws__N12_cryptography__N15_dbEncryptionSdk__N8_dynamoDb__N4_json__S12_ParsedHeader__M16_algorithmSuiteId(software.amazon.cryptography.materialproviders.internaldafny.types._IDBEAlgorithmSuiteId value)
     {
@@ -490,51 +406,29 @@ namespace AWS.Cryptography.DbEncryptionSDK.DynamoDb.Json
     {
       return ToDafny_N3_aws__N12_cryptography__N17_materialProviders__S17_EncryptionContext(value);
     }
-    public static string FromDafny_N3_aws__N12_cryptography__N15_dbEncryptionSdk__N8_dynamoDb__N4_json__S16_AttributeActions__M3_key(Dafny.ISequence<char> value)
+    public static string FromDafny_N3_aws__N12_cryptography__N15_dbEncryptionSdk__N8_dynamoDb__N4_json__S13_MemberActions__M3_key(Dafny.ISequence<char> value)
     {
       return FromDafny_N6_smithy__N3_api__S6_String(value);
     }
-    public static Dafny.ISequence<char> ToDafny_N3_aws__N12_cryptography__N15_dbEncryptionSdk__N8_dynamoDb__N4_json__S16_AttributeActions__M3_key(string value)
+    public static Dafny.ISequence<char> ToDafny_N3_aws__N12_cryptography__N15_dbEncryptionSdk__N8_dynamoDb__N4_json__S13_MemberActions__M3_key(string value)
     {
       return ToDafny_N6_smithy__N3_api__S6_String(value);
     }
-    public static AWS.Cryptography.DbEncryptionSDK.DynamoDb.Json.Action FromDafny_N3_aws__N12_cryptography__N15_dbEncryptionSdk__N8_dynamoDb__N4_json__S16_AttributeActions__M5_value(software.amazon.cryptography.dbencryptionsdk.dynamodb.json.internaldafny.types._IAction value)
+    public static AWS.Cryptography.DbEncryptionSDK.DynamoDb.Json.Action FromDafny_N3_aws__N12_cryptography__N15_dbEncryptionSdk__N8_dynamoDb__N4_json__S13_MemberActions__M5_value(software.amazon.cryptography.dbencryptionsdk.dynamodb.json.internaldafny.types._IAction value)
     {
       return FromDafny_N3_aws__N12_cryptography__N15_dbEncryptionSdk__N8_dynamoDb__N4_json__S6_Action(value);
     }
-    public static software.amazon.cryptography.dbencryptionsdk.dynamodb.json.internaldafny.types._IAction ToDafny_N3_aws__N12_cryptography__N15_dbEncryptionSdk__N8_dynamoDb__N4_json__S16_AttributeActions__M5_value(AWS.Cryptography.DbEncryptionSDK.DynamoDb.Json.Action value)
+    public static software.amazon.cryptography.dbencryptionsdk.dynamodb.json.internaldafny.types._IAction ToDafny_N3_aws__N12_cryptography__N15_dbEncryptionSdk__N8_dynamoDb__N4_json__S13_MemberActions__M5_value(AWS.Cryptography.DbEncryptionSDK.DynamoDb.Json.Action value)
     {
       return ToDafny_N3_aws__N12_cryptography__N15_dbEncryptionSdk__N8_dynamoDb__N4_json__S6_Action(value);
     }
-    public static string FromDafny_N3_aws__N12_cryptography__N15_dbEncryptionSdk__N8_dynamoDb__N4_json__S17_AttributeNameList__M6_member(Dafny.ISequence<char> value)
+    public static string FromDafny_N3_aws__N12_cryptography__N15_dbEncryptionSdk__N8_dynamoDb__N4_json__S14_MemberNameList__M6_member(Dafny.ISequence<char> value)
     {
       return FromDafny_N6_smithy__N3_api__S6_String(value);
     }
-    public static Dafny.ISequence<char> ToDafny_N3_aws__N12_cryptography__N15_dbEncryptionSdk__N8_dynamoDb__N4_json__S17_AttributeNameList__M6_member(string value)
+    public static Dafny.ISequence<char> ToDafny_N3_aws__N12_cryptography__N15_dbEncryptionSdk__N8_dynamoDb__N4_json__S14_MemberNameList__M6_member(string value)
     {
       return ToDafny_N6_smithy__N3_api__S6_String(value);
-    }
-    public static System.Collections.Generic.Dictionary<string, string> FromDafny_N3_aws__N12_cryptography__N17_materialProviders__S17_EncryptionContext(Dafny.IMap<Dafny.ISequence<byte>, Dafny.ISequence<byte>> value)
-    {
-      return value.ItemEnumerable.ToDictionary(pair => FromDafny_N3_aws__N12_cryptography__N17_materialProviders__S17_EncryptionContext__M3_key(pair.Car), pair => FromDafny_N3_aws__N12_cryptography__N17_materialProviders__S17_EncryptionContext__M5_value(pair.Cdr));
-    }
-    public static Dafny.IMap<Dafny.ISequence<byte>, Dafny.ISequence<byte>> ToDafny_N3_aws__N12_cryptography__N17_materialProviders__S17_EncryptionContext(System.Collections.Generic.Dictionary<string, string> value)
-    {
-      return Dafny.Map<Dafny.ISequence<byte>, Dafny.ISequence<byte>>.FromCollection(value.Select(pair =>
-         new Dafny.Pair<Dafny.ISequence<byte>, Dafny.ISequence<byte>>(ToDafny_N3_aws__N12_cryptography__N17_materialProviders__S17_EncryptionContext__M3_key(pair.Key), ToDafny_N3_aws__N12_cryptography__N17_materialProviders__S17_EncryptionContext__M5_value(pair.Value))
-     ));
-    }
-    public static AWS.Cryptography.MaterialProviders.ICryptographicMaterialsManager FromDafny_N3_aws__N12_cryptography__N17_materialProviders__S38_CryptographicMaterialsManagerReference(software.amazon.cryptography.materialproviders.internaldafny.types.ICryptographicMaterialsManager value)
-    {
-      // This is converting a reference type in a dependant module.
-      // Therefore it defers to the dependant module for conversion
-      return AWS.Cryptography.MaterialProviders.TypeConversion.FromDafny_N3_aws__N12_cryptography__N17_materialProviders__S38_CryptographicMaterialsManagerReference(value);
-    }
-    public static software.amazon.cryptography.materialproviders.internaldafny.types.ICryptographicMaterialsManager ToDafny_N3_aws__N12_cryptography__N17_materialProviders__S38_CryptographicMaterialsManagerReference(AWS.Cryptography.MaterialProviders.ICryptographicMaterialsManager value)
-    {
-      // This is converting a reference type in a dependant module.
-      // Therefore it defers to the dependant module for conversion
-      return AWS.Cryptography.MaterialProviders.TypeConversion.ToDafny_N3_aws__N12_cryptography__N17_materialProviders__S38_CryptographicMaterialsManagerReference(value);
     }
     public static AWS.Cryptography.MaterialProviders.IKeyring FromDafny_N3_aws__N12_cryptography__N17_materialProviders__S16_KeyringReference(software.amazon.cryptography.materialproviders.internaldafny.types.IKeyring value)
     {
@@ -548,43 +442,17 @@ namespace AWS.Cryptography.DbEncryptionSDK.DynamoDb.Json
       // Therefore it defers to the dependant module for conversion
       return AWS.Cryptography.MaterialProviders.TypeConversion.ToDafny_N3_aws__N12_cryptography__N17_materialProviders__S16_KeyringReference(value);
     }
-    public static AWS.Cryptography.MaterialProviders.ESDKAlgorithmSuiteId FromDafny_N3_aws__N12_cryptography__N17_materialProviders__S20_ESDKAlgorithmSuiteId(software.amazon.cryptography.materialproviders.internaldafny.types._IESDKAlgorithmSuiteId value)
+    public static AWS.Cryptography.MaterialProviders.ICryptographicMaterialsManager FromDafny_N3_aws__N12_cryptography__N17_materialProviders__S38_CryptographicMaterialsManagerReference(software.amazon.cryptography.materialproviders.internaldafny.types.ICryptographicMaterialsManager value)
     {
-      if (value.is_ALG__AES__128__GCM__IV12__TAG16__NO__KDF) return AWS.Cryptography.MaterialProviders.ESDKAlgorithmSuiteId.ALG_AES_128_GCM_IV12_TAG16_NO_KDF;
-      if (value.is_ALG__AES__192__GCM__IV12__TAG16__NO__KDF) return AWS.Cryptography.MaterialProviders.ESDKAlgorithmSuiteId.ALG_AES_192_GCM_IV12_TAG16_NO_KDF;
-      if (value.is_ALG__AES__256__GCM__IV12__TAG16__NO__KDF) return AWS.Cryptography.MaterialProviders.ESDKAlgorithmSuiteId.ALG_AES_256_GCM_IV12_TAG16_NO_KDF;
-      if (value.is_ALG__AES__128__GCM__IV12__TAG16__HKDF__SHA256) return AWS.Cryptography.MaterialProviders.ESDKAlgorithmSuiteId.ALG_AES_128_GCM_IV12_TAG16_HKDF_SHA256;
-      if (value.is_ALG__AES__192__GCM__IV12__TAG16__HKDF__SHA256) return AWS.Cryptography.MaterialProviders.ESDKAlgorithmSuiteId.ALG_AES_192_GCM_IV12_TAG16_HKDF_SHA256;
-      if (value.is_ALG__AES__256__GCM__IV12__TAG16__HKDF__SHA256) return AWS.Cryptography.MaterialProviders.ESDKAlgorithmSuiteId.ALG_AES_256_GCM_IV12_TAG16_HKDF_SHA256;
-      if (value.is_ALG__AES__128__GCM__IV12__TAG16__HKDF__SHA256__ECDSA__P256) return AWS.Cryptography.MaterialProviders.ESDKAlgorithmSuiteId.ALG_AES_128_GCM_IV12_TAG16_HKDF_SHA256_ECDSA_P256;
-      if (value.is_ALG__AES__192__GCM__IV12__TAG16__HKDF__SHA384__ECDSA__P384) return AWS.Cryptography.MaterialProviders.ESDKAlgorithmSuiteId.ALG_AES_192_GCM_IV12_TAG16_HKDF_SHA384_ECDSA_P384;
-      if (value.is_ALG__AES__256__GCM__IV12__TAG16__HKDF__SHA384__ECDSA__P384) return AWS.Cryptography.MaterialProviders.ESDKAlgorithmSuiteId.ALG_AES_256_GCM_IV12_TAG16_HKDF_SHA384_ECDSA_P384;
-      if (value.is_ALG__AES__256__GCM__HKDF__SHA512__COMMIT__KEY) return AWS.Cryptography.MaterialProviders.ESDKAlgorithmSuiteId.ALG_AES_256_GCM_HKDF_SHA512_COMMIT_KEY;
-      if (value.is_ALG__AES__256__GCM__HKDF__SHA512__COMMIT__KEY__ECDSA__P384) return AWS.Cryptography.MaterialProviders.ESDKAlgorithmSuiteId.ALG_AES_256_GCM_HKDF_SHA512_COMMIT_KEY_ECDSA_P384;
-      throw new System.ArgumentException("Invalid AWS.Cryptography.MaterialProviders.ESDKAlgorithmSuiteId value");
+      // This is converting a reference type in a dependant module.
+      // Therefore it defers to the dependant module for conversion
+      return AWS.Cryptography.MaterialProviders.TypeConversion.FromDafny_N3_aws__N12_cryptography__N17_materialProviders__S38_CryptographicMaterialsManagerReference(value);
     }
-    public static software.amazon.cryptography.materialproviders.internaldafny.types._IESDKAlgorithmSuiteId ToDafny_N3_aws__N12_cryptography__N17_materialProviders__S20_ESDKAlgorithmSuiteId(AWS.Cryptography.MaterialProviders.ESDKAlgorithmSuiteId value)
+    public static software.amazon.cryptography.materialproviders.internaldafny.types.ICryptographicMaterialsManager ToDafny_N3_aws__N12_cryptography__N17_materialProviders__S38_CryptographicMaterialsManagerReference(AWS.Cryptography.MaterialProviders.ICryptographicMaterialsManager value)
     {
-      if (AWS.Cryptography.MaterialProviders.ESDKAlgorithmSuiteId.ALG_AES_128_GCM_IV12_TAG16_NO_KDF.Equals(value)) return software.amazon.cryptography.materialproviders.internaldafny.types.ESDKAlgorithmSuiteId.create_ALG__AES__128__GCM__IV12__TAG16__NO__KDF();
-      if (AWS.Cryptography.MaterialProviders.ESDKAlgorithmSuiteId.ALG_AES_192_GCM_IV12_TAG16_NO_KDF.Equals(value)) return software.amazon.cryptography.materialproviders.internaldafny.types.ESDKAlgorithmSuiteId.create_ALG__AES__192__GCM__IV12__TAG16__NO__KDF();
-      if (AWS.Cryptography.MaterialProviders.ESDKAlgorithmSuiteId.ALG_AES_256_GCM_IV12_TAG16_NO_KDF.Equals(value)) return software.amazon.cryptography.materialproviders.internaldafny.types.ESDKAlgorithmSuiteId.create_ALG__AES__256__GCM__IV12__TAG16__NO__KDF();
-      if (AWS.Cryptography.MaterialProviders.ESDKAlgorithmSuiteId.ALG_AES_128_GCM_IV12_TAG16_HKDF_SHA256.Equals(value)) return software.amazon.cryptography.materialproviders.internaldafny.types.ESDKAlgorithmSuiteId.create_ALG__AES__128__GCM__IV12__TAG16__HKDF__SHA256();
-      if (AWS.Cryptography.MaterialProviders.ESDKAlgorithmSuiteId.ALG_AES_192_GCM_IV12_TAG16_HKDF_SHA256.Equals(value)) return software.amazon.cryptography.materialproviders.internaldafny.types.ESDKAlgorithmSuiteId.create_ALG__AES__192__GCM__IV12__TAG16__HKDF__SHA256();
-      if (AWS.Cryptography.MaterialProviders.ESDKAlgorithmSuiteId.ALG_AES_256_GCM_IV12_TAG16_HKDF_SHA256.Equals(value)) return software.amazon.cryptography.materialproviders.internaldafny.types.ESDKAlgorithmSuiteId.create_ALG__AES__256__GCM__IV12__TAG16__HKDF__SHA256();
-      if (AWS.Cryptography.MaterialProviders.ESDKAlgorithmSuiteId.ALG_AES_128_GCM_IV12_TAG16_HKDF_SHA256_ECDSA_P256.Equals(value)) return software.amazon.cryptography.materialproviders.internaldafny.types.ESDKAlgorithmSuiteId.create_ALG__AES__128__GCM__IV12__TAG16__HKDF__SHA256__ECDSA__P256();
-      if (AWS.Cryptography.MaterialProviders.ESDKAlgorithmSuiteId.ALG_AES_192_GCM_IV12_TAG16_HKDF_SHA384_ECDSA_P384.Equals(value)) return software.amazon.cryptography.materialproviders.internaldafny.types.ESDKAlgorithmSuiteId.create_ALG__AES__192__GCM__IV12__TAG16__HKDF__SHA384__ECDSA__P384();
-      if (AWS.Cryptography.MaterialProviders.ESDKAlgorithmSuiteId.ALG_AES_256_GCM_IV12_TAG16_HKDF_SHA384_ECDSA_P384.Equals(value)) return software.amazon.cryptography.materialproviders.internaldafny.types.ESDKAlgorithmSuiteId.create_ALG__AES__256__GCM__IV12__TAG16__HKDF__SHA384__ECDSA__P384();
-      if (AWS.Cryptography.MaterialProviders.ESDKAlgorithmSuiteId.ALG_AES_256_GCM_HKDF_SHA512_COMMIT_KEY.Equals(value)) return software.amazon.cryptography.materialproviders.internaldafny.types.ESDKAlgorithmSuiteId.create_ALG__AES__256__GCM__HKDF__SHA512__COMMIT__KEY();
-      if (AWS.Cryptography.MaterialProviders.ESDKAlgorithmSuiteId.ALG_AES_256_GCM_HKDF_SHA512_COMMIT_KEY_ECDSA_P384.Equals(value)) return software.amazon.cryptography.materialproviders.internaldafny.types.ESDKAlgorithmSuiteId.create_ALG__AES__256__GCM__HKDF__SHA512__COMMIT__KEY__ECDSA__P384();
-      throw new System.ArgumentException("Invalid AWS.Cryptography.MaterialProviders.ESDKAlgorithmSuiteId value");
-    }
-    public static long FromDafny_N3_aws__N12_cryptography__N15_dbEncryptionSdk__N8_dynamoDb__N4_json__S11_FrameLength(long value)
-    {
-      return value;
-    }
-    public static long ToDafny_N3_aws__N12_cryptography__N15_dbEncryptionSdk__N8_dynamoDb__N4_json__S11_FrameLength(long value)
-    {
-      return value;
+      // This is converting a reference type in a dependant module.
+      // Therefore it defers to the dependant module for conversion
+      return AWS.Cryptography.MaterialProviders.TypeConversion.ToDafny_N3_aws__N12_cryptography__N17_materialProviders__S38_CryptographicMaterialsManagerReference(value);
     }
     public static AWS.Cryptography.MaterialProviders.DBEAlgorithmSuiteId FromDafny_N3_aws__N12_cryptography__N17_materialProviders__S19_DBEAlgorithmSuiteId(software.amazon.cryptography.materialproviders.internaldafny.types._IDBEAlgorithmSuiteId value)
     {
@@ -598,14 +466,14 @@ namespace AWS.Cryptography.DbEncryptionSDK.DynamoDb.Json
       if (AWS.Cryptography.MaterialProviders.DBEAlgorithmSuiteId.ALG_AES_256_GCM_HKDF_SHA512_COMMIT_KEY_ECDSA_P384_SYMSIG_HMAC_SHA384.Equals(value)) return software.amazon.cryptography.materialproviders.internaldafny.types.DBEAlgorithmSuiteId.create_ALG__AES__256__GCM__HKDF__SHA512__COMMIT__KEY__ECDSA__P384__SYMSIG__HMAC__SHA384();
       throw new System.ArgumentException("Invalid AWS.Cryptography.MaterialProviders.DBEAlgorithmSuiteId value");
     }
-    public static System.Collections.Generic.Dictionary<string, string> FromDafny_N3_aws__N12_cryptography__N15_dbEncryptionSdk__N8_dynamoDb__N4_json__S12_SignedValues(Dafny.IMap<Dafny.ISequence<char>, Dafny.ISequence<char>> value)
+    public static System.Collections.Generic.Dictionary<string, string> FromDafny_N3_aws__N12_cryptography__N17_materialProviders__S17_EncryptionContext(Dafny.IMap<Dafny.ISequence<byte>, Dafny.ISequence<byte>> value)
     {
-      return value.ItemEnumerable.ToDictionary(pair => FromDafny_N3_aws__N12_cryptography__N15_dbEncryptionSdk__N8_dynamoDb__N4_json__S12_SignedValues__M3_key(pair.Car), pair => FromDafny_N3_aws__N12_cryptography__N15_dbEncryptionSdk__N8_dynamoDb__N4_json__S12_SignedValues__M5_value(pair.Cdr));
+      return value.ItemEnumerable.ToDictionary(pair => FromDafny_N3_aws__N12_cryptography__N17_materialProviders__S17_EncryptionContext__M3_key(pair.Car), pair => FromDafny_N3_aws__N12_cryptography__N17_materialProviders__S17_EncryptionContext__M5_value(pair.Cdr));
     }
-    public static Dafny.IMap<Dafny.ISequence<char>, Dafny.ISequence<char>> ToDafny_N3_aws__N12_cryptography__N15_dbEncryptionSdk__N8_dynamoDb__N4_json__S12_SignedValues(System.Collections.Generic.Dictionary<string, string> value)
+    public static Dafny.IMap<Dafny.ISequence<byte>, Dafny.ISequence<byte>> ToDafny_N3_aws__N12_cryptography__N17_materialProviders__S17_EncryptionContext(System.Collections.Generic.Dictionary<string, string> value)
     {
-      return Dafny.Map<Dafny.ISequence<char>, Dafny.ISequence<char>>.FromCollection(value.Select(pair =>
-         new Dafny.Pair<Dafny.ISequence<char>, Dafny.ISequence<char>>(ToDafny_N3_aws__N12_cryptography__N15_dbEncryptionSdk__N8_dynamoDb__N4_json__S12_SignedValues__M3_key(pair.Key), ToDafny_N3_aws__N12_cryptography__N15_dbEncryptionSdk__N8_dynamoDb__N4_json__S12_SignedValues__M5_value(pair.Value))
+      return Dafny.Map<Dafny.ISequence<byte>, Dafny.ISequence<byte>>.FromCollection(value.Select(pair =>
+         new Dafny.Pair<Dafny.ISequence<byte>, Dafny.ISequence<byte>>(ToDafny_N3_aws__N12_cryptography__N17_materialProviders__S17_EncryptionContext__M3_key(pair.Key), ToDafny_N3_aws__N12_cryptography__N17_materialProviders__S17_EncryptionContext__M5_value(pair.Value))
      ));
     }
     public static System.Collections.Generic.List<AWS.Cryptography.MaterialProviders.EncryptedDataKey> FromDafny_N3_aws__N12_cryptography__N17_materialProviders__S20_EncryptedDataKeyList(Dafny.ISequence<software.amazon.cryptography.materialproviders.internaldafny.types._IEncryptedDataKey> value)
@@ -631,22 +499,6 @@ namespace AWS.Cryptography.DbEncryptionSDK.DynamoDb.Json
     public static Dafny.ISequence<byte> ToDafny_N3_aws__N12_cryptography__N17_materialProviders__S17_EncryptionContext__M5_value(string value)
     {
       return ToDafny_N3_aws__N12_cryptography__N17_materialProviders__S9_Utf8Bytes(value);
-    }
-    public static string FromDafny_N3_aws__N12_cryptography__N15_dbEncryptionSdk__N8_dynamoDb__N4_json__S12_SignedValues__M3_key(Dafny.ISequence<char> value)
-    {
-      return FromDafny_N6_smithy__N3_api__S6_String(value);
-    }
-    public static Dafny.ISequence<char> ToDafny_N3_aws__N12_cryptography__N15_dbEncryptionSdk__N8_dynamoDb__N4_json__S12_SignedValues__M3_key(string value)
-    {
-      return ToDafny_N6_smithy__N3_api__S6_String(value);
-    }
-    public static string FromDafny_N3_aws__N12_cryptography__N15_dbEncryptionSdk__N8_dynamoDb__N4_json__S12_SignedValues__M5_value(Dafny.ISequence<char> value)
-    {
-      return FromDafny_N6_smithy__N3_api__S6_String(value);
-    }
-    public static Dafny.ISequence<char> ToDafny_N3_aws__N12_cryptography__N15_dbEncryptionSdk__N8_dynamoDb__N4_json__S12_SignedValues__M5_value(string value)
-    {
-      return ToDafny_N6_smithy__N3_api__S6_String(value);
     }
     public static AWS.Cryptography.MaterialProviders.EncryptedDataKey FromDafny_N3_aws__N12_cryptography__N17_materialProviders__S20_EncryptedDataKeyList__M6_member(software.amazon.cryptography.materialproviders.internaldafny.types._IEncryptedDataKey value)
     {
